closure up to induction again skipped old faiils

theories/Logic/fol.v
@@ -960,3 +960,219 @@ Proof.
 intros. unfold closure. rewrite closure_closed'; auto.
 Qed.
 
+Lemma closure_type_lor : forall (L : list nat) (A B : formula) (t : term), closed_t t = true -> closure_type (lor A B) t L = lor (closure_type A t L) (closure_type B t L).
+Proof.
+intros L. induction L. auto. intros. simpl. apply IHL. auto.
+Qed.
+
+Lemma closure_closed_id : forall (A : formula) (t : term), closed A = true -> closure A t = A.
+intros. unfold closure. rewrite closed_free_list; auto.
+Qed.
+
+Lemma closure_closed_list_id : forall (L : list nat) (A : formula) (t : term), closed A = true -> closure_type A t L = A.
+intros L. induction L; auto. intros. simpl. rewrite closed_subst_eq; auto. 
+Qed.
+
+Lemma closure_type_symm : forall (A : formula) (t : term) (n m : nat) (L : list nat), closed_t t = true -> closure_type A t (n :: m :: L) = closure_type A t (m :: n :: L).
+Proof.
+intros. case (eq_nat m n) eqn:X.
+- apply nat_eq_decid in X. destruct X. auto.
+- simpl. rewrite substitution_order; auto.
+Qed.
+
+Lemma closure_type_concat_symm : forall (L1 L2 : list nat) (A : formula) (t : term), closed_t t = true -> closure_type A t (concat L1 L2) = closure_type A t (concat L2 L1).
+Proof.
+intros L1. induction L1.
+- intros. simpl. rewrite concat_empty_right. auto.
+- intros L2. simpl. induction L2; intros.
+  + simpl. rewrite concat_empty_right. auto.
+  + rewrite IHL1; auto. simpl. rewrite <- IHL2; auto. rewrite IHL1; auto. case (eq_nat x0 x) eqn:X.
+   * apply nat_eq_decid in X. destruct X. auto.
+   * rewrite substitution_order; auto.
+Qed.
+
+Lemma closure_type_concat : forall (L1 L2 : list nat) (A : formula) (t : term), closed_t t = true -> closure_type A t (concat L1 L2) = closure_type (closure_type A t L1) t L2.
+Proof.
+intros L1. induction L1. auto. intros. simpl. rewrite IHL1; auto.
+Qed.
+
+
+Lemma closure_type_not_used : forall (L : list nat) (A : formula) (t : term) (n : nat), closed_t t = true -> member n (free_list A) = false -> closure_type A t (n :: L) = closure_type A t L.
+Proof.
+intros L. induction L.
+- intros. simpl. apply closed_subst_eq_aux. auto.
+- intros. simpl. case (eq_nat x n) eqn:X.
+  + apply nat_eq_decid in X. destruct X. repeat rewrite (closed_subst_eq_aux _ _ _ H0). auto.
+  + rewrite substitution_order; auto. rewrite closed_subst_eq_aux. auto. rewrite subst_remove; auto. apply remove_member_false. auto.
+Qed.
+
+Lemma closure_type_not_used_any : forall (L1 L2 : list nat) (A : formula) (t : term) (n : nat), closed_t t = true -> member n (free_list A) = false -> closure_type A t (concat L1 (n :: L2)) = closure_type A t (concat L1 L2).
+Proof.
+intros. rewrite (closure_type_concat_symm _ L2); auto. rewrite closure_type_concat_symm; auto. apply closure_type_not_used; auto.
+Qed.
+
+Lemma closure_type_not_used_remove : forall (L : list nat) (A : formula) (t : term) (n : nat), closed_t t = true -> member n (free_list A) = false -> closure_type A t (remove n L) = closure_type A t L.
+Proof.
+intros L. induction L. auto. intros. simpl. case (eq_nat x n) eqn:X.
+- apply nat_eq_decid in X. destruct X. rewrite IHL; auto. rewrite closed_subst_eq_aux; auto.
+- simpl. rewrite IHL; auto. rewrite subst_remove; auto. apply remove_member_false. auto.
+Qed.
+
+Lemma closure_type_dupes : forall (L : list nat) (A : formula) (t : term), closed_t t = true -> closure_type A t L = closure_type A t (remove_dups L).
+Proof.
+intros L. induction L. auto. intros. simpl. rewrite IHL; auto. rewrite closure_type_not_used_remove; auto. rewrite subst_remove; auto. apply remove_not_member.
+Qed.
+
+Lemma closure_lor : forall A B t, closed_t t = true -> closure (lor A B) t = lor (closure A t) (closure B t).
+Proof.
+intros A. unfold closure. simpl. induction (free_list A) eqn:X.
+- intros. simpl. rewrite <- free_list_remove_dups. rewrite closure_type_lor; auto. rewrite closure_closed_list_id; auto. apply free_list_closed. auto.
+- intros. rewrite <- closure_type_dupes; auto. rewrite closure_type_lor; auto. rewrite closure_type_concat; auto. rewrite closure_type_concat_symm; auto. rewrite closure_type_concat; auto.
+  destruct X. rewrite closure_closed_list_id. rewrite (closure_closed_list_id (free_list A) (closure_type B t (free_list B))). auto. apply closure_closed; auto. apply closure_closed; auto.
+Qed.
+
+Lemma closure_neg_list : forall L A t, closed_t t = true -> closure_type (neg A) t L = neg (closure_type A t L).
+Proof.
+intros L. induction L. auto. intros. simpl. rewrite IHL; auto.
+Qed.
+
+Lemma closure_univ_list : forall L A t n, closed_t t = true -> closure_type (univ n A) t L = univ n (closure_type A t (remove n L)).
+Proof.
+intros L. induction L. auto. intros. simpl. case (eq_nat n x) eqn:X.
+- apply eq_nat_symm in X. rewrite X. auto.
+- rewrite IHL; auto. apply eq_nat_symm' in X. rewrite X. auto.
+Qed.
+
+Lemma closure_neg : forall A t, closed_t t = true -> closure (neg A) t = neg (closure A t).
+Proof.
+intros. apply closure_neg_list. auto.
+Qed.
+
+Lemma closure_univ : forall A t n, closed_t t = true -> closure (univ n A) t = univ n (closure_type A t (free_list (univ n A))).
+Proof.
+intros. unfold closure. simpl. rewrite <- remove_twice at 2. apply closure_univ_list. auto.
+Qed.
+
+Lemma num_conn_closure_eq_list : forall (L : list nat) (A : formula) (t : term), num_conn A = num_conn (closure_type A t L).
+Proof.
+intros L. induction L. auto. intros. simpl. rewrite <- IHL. rewrite num_conn_sub. auto.
+Qed.
+
+Lemma num_conn_closure_eq : forall (A : formula) (t : term), num_conn A = num_conn (closure A t).
+Proof.
+intros. apply num_conn_closure_eq_list.
+Qed.
+
+Lemma closure_subst_list :  forall (L : list nat) (A : formula) (t s : term) (n : nat), closed_t t = true -> closed_t s = true -> (substitution (closure_type A t (remove n L)) n s) = (closure_type (substitution A n s) t L).
+Proof.
+intros L. induction L. auto. intros. simpl. case (eq_nat x n) eqn:X.
+- apply nat_eq_decid in X. destruct X. rewrite IHL; auto. rewrite (closed_subst_eq_aux (substitution A x s)). auto. rewrite subst_remove; auto. apply remove_not_member.
+- simpl. rewrite IHL; auto. apply eq_nat_symm' in X. rewrite substitution_order; auto.
+Qed.
+
+Lemma closure_subst :  forall (A : formula) (t s : term) (n : nat), closed_t t = true -> closed_t s = true -> (substitution (closure_type A t (free_list (univ n A))) n s) = (closure (substitution A n s) t).
+Proof.
+intros. unfold closure. rewrite <- closure_subst_list; auto. rewrite remove_not_mem_idem. rewrite (free_list_univ_sub _ _ _ (free_list (univ n A))); auto. rewrite subst_remove; auto. apply remove_not_member.
+Qed.
+
+Fixpoint closure_type_t (t s : term) (L : list nat) : term :=
+match L with
+| [] => t
+| x :: L' => closure_type_t (substitution_t t x s) s L'
+end.
+
+Definition closure_t (t s : term) := closure_type_t t s (free_list_t t).
+
+Lemma closure_closed_t' : forall (L : list nat) (t s : term), closed_t s = true -> free_list_t t = L -> closed_t (closure_type_t t s L) = true.
+Proof.
+intros L. induction L; intros.
+- simpl. apply free_list_closed_t. auto.
+- simpl. rewrite IHL; auto. rewrite subst_remove_t; auto. rewrite H0. rewrite remove_dups_idem_remove_triv. auto. destruct H0. rewrite <- free_list_remove_dups_t. auto.
+Qed.
+
+Lemma closure_closed_t : forall (t s : term), closed_t s = true -> closed_t (closure_t t s) = true.
+Proof.
+intros. unfold closure_t. rewrite closure_closed_t'; auto.
+Qed.
+
+Lemma closure_type_equiv_list : forall L t1 t2 s, closure_type (atom (equ t1 t2)) s L = atom (equ (closure_type_t t1 s L) (closure_type_t t2 s L)).
+Proof.
+intros L. induction L; simpl; auto.
+Qed.
+
+Lemma closure_type_concat_t : forall (L1 L2 : list nat) (t s : term), closed_t s = true -> closure_type_t t s (concat L1 L2) = closure_type_t (closure_type_t t s L1) s L2.
+Proof.
+intros L1. induction L1. auto. intros. simpl. rewrite IHL1; auto.
+Qed.
+
+Lemma closure_type_concat_symm_t : forall (L1 L2 : list nat) (t s : term), closed_t s = true -> closure_type_t t s (concat L1 L2) = closure_type_t t s (concat L2 L1).
+Proof.
+intros L1. induction L1.
+- intros. simpl. rewrite concat_empty_right. auto.
+- intros L2. simpl. induction L2; intros.
+  + simpl. rewrite concat_empty_right. auto.
+  + rewrite IHL1; auto. simpl. rewrite <- IHL2; auto. rewrite IHL1; auto. case (eq_nat x0 x) eqn:X.
+   * apply nat_eq_decid in X. destruct X. auto.
+   * rewrite substitution_order_t; auto.
+Qed.
+
+Lemma closure_closed_id_t : forall (t s : term), closed_t t = true -> closure_t t s = t.
+intros. unfold closure_t. rewrite closed_free_list_t; auto.
+Qed.
+
+Lemma closure_closed_list_id_t : forall (L : list nat) (t s : term), closed_t t = true -> closure_type_t t s L = t.
+intros L. induction L; auto. intros. simpl. rewrite closed_subst_eq_t; auto. 
+Qed.
+
+Lemma closure_type_not_used_remove_t : forall (L : list nat) (t s : term) (n : nat), closed_t s = true -> member n (free_list_t t) = false -> closure_type_t t s (remove n L) = closure_type_t t s L.
+Proof.
+intros L. induction L. auto. intros. simpl. case (eq_nat x n) eqn:X.
+- apply nat_eq_decid in X. destruct X. rewrite IHL; auto. rewrite closed_subst_eq_aux_t; auto.
+- simpl. rewrite IHL; auto. rewrite subst_remove_t; auto. apply remove_member_false. auto.
+Qed.
+
+Lemma closure_type_dupes_t : forall (L : list nat) (t s : term), closed_t s = true -> closure_type_t t s L = closure_type_t t s (remove_dups L).
+Proof.
+intros L. induction L. auto. intros. simpl. rewrite IHL; auto. rewrite closure_type_not_used_remove_t; auto. rewrite subst_remove_t; auto. apply remove_not_member.
+Qed.
+
+Lemma closure_type_equiv : forall t1 t2 s, closed_t s = true -> closure (atom (equ t1 t2)) s = atom (equ (closure_t t1 s) (closure_t t2 s)).
+Proof.
+intros. unfold closure. rewrite closure_type_equiv_list. simpl. rewrite <- closure_type_dupes_t; auto. rewrite <- closure_type_dupes_t; auto.
+rewrite closure_type_concat_t; auto. rewrite closure_type_concat_symm_t; auto. rewrite closure_type_concat_t; auto.
+rewrite (closure_closed_list_id_t (free_list_t t2)). rewrite (closure_closed_list_id_t (free_list_t t1) (closure_type_t t2 s _)); auto. apply closure_closed_t; auto. apply closure_closed_t; auto.
+Qed.
+
+Lemma closure_t_succ_list : forall L t s, closure_type_t (succ t) s L = succ (closure_type_t t s L).
+Proof.
+intros L. induction L. auto. intros. simpl. rewrite IHL. auto.
+Qed.
+
+Lemma closure_t_succ : forall t s, closure_t (succ t) s = succ (closure_t t s).
+Proof.
+intros. apply closure_t_succ_list.
+Qed.
+
+Lemma closure_t_plus_list : forall L t1 t2 s, closure_type_t (plus t1 t2) s L = plus (closure_type_t t1 s L) (closure_type_t t2 s L).
+Proof.
+intros L. induction L. auto. intros. simpl. rewrite IHL. auto.
+Qed.
+
+Lemma closure_t_plus : forall t1 t2 s, closed_t s = true -> closure_t (plus t1 t2) s = plus (closure_t t1 s) (closure_t t2 s).
+Proof.
+intros. unfold closure_t. rewrite closure_t_plus_list. simpl. rewrite <- closure_type_dupes_t; auto. rewrite <- closure_type_dupes_t; auto.
+rewrite closure_type_concat_t; auto. rewrite closure_type_concat_symm_t; auto. rewrite closure_type_concat_t; auto.
+rewrite (closure_closed_list_id_t (free_list_t t2)). rewrite (closure_closed_list_id_t (free_list_t t1) (closure_type_t t2 s _)); auto. apply closure_closed_t; auto. apply closure_closed_t; auto.
+Qed.
+
+Lemma closure_t_times_list : forall L t1 t2 s, closure_type_t (times t1 t2) s L = times (closure_type_t t1 s L) (closure_type_t t2 s L).
+Proof.
+intros L. induction L. auto. intros. simpl. rewrite IHL. auto.
+Qed.
+
+Lemma closure_t_times : forall t1 t2 s, closed_t s = true -> closure_t (times t1 t2) s = times (closure_t t1 s) (closure_t t2 s).
+Proof.
+intros. unfold closure_t. rewrite closure_t_times_list. simpl. rewrite <- closure_type_dupes_t; auto. rewrite <- closure_type_dupes_t; auto.
+rewrite closure_type_concat_t; auto. rewrite closure_type_concat_symm_t; auto. rewrite closure_type_concat_t; auto.
+rewrite (closure_closed_list_id_t (free_list_t t2)). rewrite (closure_closed_list_id_t (free_list_t t1) (closure_type_t t2 s _)); auto. apply closure_closed_t; auto. apply closure_closed_t; auto.
+Qed.
